wip: continue linking high-level and low-level specs

code/experimental/rsapss/Hacl.Spec.Bignum.Exponentiation.fst
@@ -12,6 +12,9 @@ open Hacl.Spec.Bignum.Montgomery
 open Hacl.Spec.Bignum.Montgomery.PreCompConstants
 
 
+module M = Hacl.Spec.Bignum.Montgomery.Lemmas
+module BL = Hacl.Spec.Bignum.Lemmas
+
 #reset-options "--z3rlimit 50 --max_fuel 0 --max_ifuel 0"
 
 val bn_is_bit_set: #len:size_nat -> input:lbignum len -> ind:size_nat{ind / 64 < len} -> bool
@@ -64,3 +67,115 @@ let mod_exp modBits nLen n r2 a bBits b =
   let accM = to_mont n nInv_u64 r2 acc in
   let (aM, accM) = repeati bBits (mod_exp_f #nLen #rLen n nInv_u64 bBits bLen b) (aM, accM) in
   from_mont n nInv_u64 accM
+
+
+val mod_exp_f_lemma:
+    #nLen:size_nat
+  -> #rLen:size_nat{rLen = nLen + 1 /\ rLen + rLen <= max_size_t}
+  -> n:lbignum nLen
+  -> mu:uint64
+  -> bBits:size_pos
+  -> bLen:size_nat{bLen == blocks bBits 64}
+  -> b:lbignum bLen
+  -> i:nat{i < bBits}
+  -> aM_accM0: tuple2 (lbignum rLen) (lbignum rLen) -> Lemma
+  (requires
+   (let (aM0, accM0) = aM_accM0 in
+    (1 + (bn_v n % pow2 64) * v mu) % pow2 64 == 0 /\
+    bn_v n % 2 = 1 /\ 1 < bn_v n /\ bn_v n < pow2 (64 * nLen) /\
+    0 < bn_v b /\ bn_v b < pow2 bBits /\
+    bn_v aM0 < 2 * bn_v n /\ bn_v accM0 < 2 * bn_v n))
+  (ensures
+   (let (aM0, accM0) = aM_accM0 in
+    let (aM1, accM1) = mod_exp_f #nLen #rLen n mu bBits bLen b i aM_accM0 in
+    let (aM2, accM2) = BL.mod_exp_f_ll rLen (bn_v n) (v mu) bBits (bn_v b) i (bn_v aM0, bn_v accM0) in
+    bn_v aM1 == aM2 /\ bn_v accM1 == accM2 /\
+    bn_v aM1 < 2 * bn_v n /\ bn_v accM1 < 2 * bn_v n))
+
+let mod_exp_f_lemma #nLen #rLen n mu bBits bLen b i (aM0, accM0) =
+  let (aM1, accM1) = mod_exp_f #nLen #rLen n mu bBits bLen b i (aM0, accM0) in
+  let (aM2, accM2) = BL.mod_exp_f_ll rLen (bn_v n) (v mu) bBits (bn_v b) i (bn_v aM0, bn_v accM0) in
+  assume (bn_v aM1 == aM2 /\ bn_v accM1 == accM2);
+  let d, k = BL.eea_pow2_odd (64 * rLen) (bn_v n) in
+  BL.mod_exp_mont_preconditions rLen (bn_v n) (v mu);
+  BL.mod_exp_mont_preconditions_rLen nLen (bn_v n);
+  BL.mod_exp_mont_ll_lemma_fits_loop_step rLen (bn_v n) d (v mu) bBits (bn_v b) i (bn_v aM0) (bn_v accM0)
+
+
+val mod_exp_mont_loop_lemma:
+    #nLen:size_nat
+  -> #rLen:size_nat{rLen = nLen + 1 /\ rLen + rLen <= max_size_t}
+  -> n:lbignum nLen
+  -> mu:uint64
+  -> bBits:size_pos
+  -> bLen:size_nat{bLen == blocks bBits 64}
+  -> b:lbignum bLen
+  -> aM_accM0: tuple2 (lbignum rLen) (lbignum rLen) -> Lemma
+  (requires
+   (let (aM0, accM0) = aM_accM0 in
+    (1 + (bn_v n % pow2 64) * v mu) % pow2 64 == 0 /\
+    bn_v n % 2 = 1 /\ 1 < bn_v n /\ bn_v n < pow2 (64 * nLen) /\
+    0 < bn_v b /\ bn_v b < pow2 bBits /\
+    bn_v aM0 < 2 * bn_v n /\ bn_v accM0 < 2 * bn_v n))
+  (ensures
+   (let (aM0, accM0) = aM_accM0 in
+    let (aM1, accM1) = repeati bBits (mod_exp_f #nLen #rLen n mu bBits bLen b) (aM0, accM0) in
+    let (aM2, accM2) = repeati bBits (BL.mod_exp_f_ll rLen (bn_v n) (v mu) bBits (bn_v b)) (bn_v aM0, bn_v accM0) in
+    bn_v aM1 == aM2 /\ bn_v accM1 == accM2 /\
+    bn_v aM1 < 2 * bn_v n /\ bn_v accM1 < 2 * bn_v n))
+
+let mod_exp_mont_loop_lemma #nLen #rLen n mu bBits bLen b (aM0, accM0) =
+  let (aM1, accM1) = repeati bBits (mod_exp_f #nLen #rLen n mu bBits bLen b) (aM0, accM0) in
+  let (aM2, accM2) = repeati bBits (BL.mod_exp_f_ll rLen (bn_v n) (v mu) bBits (bn_v b)) (bn_v aM0, bn_v accM0) in
+  assume (bn_v aM1 == aM2 /\ bn_v accM1 == accM2);
+  let d, k = BL.eea_pow2_odd (64 * rLen) (bn_v n) in
+  BL.mod_exp_mont_preconditions rLen (bn_v n) (v mu);
+  BL.mod_exp_mont_preconditions_rLen nLen (bn_v n);
+  BL.mod_exp_mont_ll_lemma_fits_loop rLen (bn_v n) d (v mu) bBits (bn_v b) bBits (bn_v aM0) (bn_v accM0)
+
+
+val mod_exp_mont_lemma:
+    modBits:size_pos
+  -> nLen:size_pos{nLen = (blocks modBits 64) /\ 128 * (nLen + 1) <= max_size_t}
+  -> n:lbignum nLen
+  -> r2:lbignum nLen
+  -> a:lbignum nLen
+  -> bBits:size_pos
+  -> b:lbignum (blocks bBits 64) -> Lemma
+  (requires
+   (bn_v n % 2 = 1 /\ 1 < bn_v n /\ bn_v n < pow2 (64 * nLen) /\
+    0 < bn_v b /\ bn_v b < pow2 bBits /\ bn_v a < bn_v n /\
+    bn_v r2 == pow2 (128 * (nLen + 1)) % bn_v n))
+  (ensures
+   (let mu = mod_inv_u64 n.[0] in
+    let res1 = mod_exp modBits nLen n r2 a bBits b in
+    let res2 = BL.mod_exp_mont_ll_final_sub (nLen + 1) (bn_v n) (v mu) (bn_v a) bBits (bn_v b) in
+    bn_v res1 == res2 /\ bn_v res1 < bn_v n))
+
+let mod_exp_mont_lemma modBits nLen n r2 a bBits b =
+  let rLen = nLen + 1 in
+  let bLen = blocks bBits 64 in
+
+  let acc  = create nLen (u64 0) in
+  let acc = acc.[0] <- u64 1 in
+  assume (bn_v acc == 1);
+
+  let mu = mod_inv_u64 n.[0] in
+  assume (v n.[0] % 2 = 1); // since bn_v n % 2 = 1
+  assume (bn_v n % pow2 64 == v n.[0]);
+  mod_inv_u64_lemma n.[0];
+
+  let aM0 = to_mont #nLen #rLen n mu r2 a in
+  to_mont_lemma #nLen #rLen n mu r2 a;
+
+  let accM0 = to_mont #nLen #rLen n mu r2 acc in
+  to_mont_lemma #nLen #rLen n mu r2 acc;
+
+  let (aM1, accM1) = repeati bBits (mod_exp_f #nLen #rLen n mu bBits bLen b) (aM0, accM0) in
+  mod_exp_mont_loop_lemma #nLen #rLen n mu bBits bLen b (aM0, accM0);
+
+  let res = from_mont n mu accM1 in
+  from_mont_lemma #nLen #rLen n mu accM1;
+  assert (bn_v res == BL.mod_exp_mont_ll rLen (bn_v n) (v mu) (bn_v a) bBits (bn_v b));
+  assert (bn_v res <= bn_v n);
+  admit() // TODO: add a final conditional substraction
